Define and verify dec_list

programs.v
@@ -7,19 +7,49 @@ Definition dec_list : val :=
     match: "l" with
     | NONE => VUnit
     | SOME "p" =>
-        let: "x" := EFst "p" in
-        let: "l" := !(ESnd "p") in
+        let: "x" := EFst !"p" in
+        let: "l" := ESnd !"p" in
         if: "x" =: 0
-          then EThrow tt 0
-          else "x" <- !"x" -: 1;;
+          then EThrow tt ()
+          else "p" <- ("x" -: 1, "l");;
                "dec_list" "l"
     end.
 
-Fixpoint is_list (v : val) (l : list nat) : sepProp :=
+Fixpoint is_list (l : list nat) (v : val) : sepProp :=
   match l with
   | [] => @[ v = NONEV ]
   | n :: l' => Ex p v',
-      @[ v = SOMEV (VRef p, v') ] **
-      p ~> VNat n **
-      is_list v' l'
+      @[ v = SOMEV (VRef p) ] **
+      p ~> (% VNat n, v' %) **
+      is_list l' v'
   end.
+
+Lemma dec_list_spec l v :
+  {{ is_list l v }}
+    dec_list v
+  {{ vret, @[ vret = () ] ** is_list (map pred l) v }}
+  {{ t vex, @[ t = tt /\ vex = () ] **
+            Ex l1 l2, @[ l = l1 ++ l2 ] **
+                      is_list (map pred l1 ++ l2) v }}.
+Proof.
+  iIntros "Hv".
+  iInduction l as [| n l'] "IH" forall (v); simpl; iApply AppRec_wp.
+  - iDestruct "Hv" as %->. iApply Match_InjL_wp. by iApply Val_wp.
+  - iDestruct "Hv" as (p v' ->) "(Hp & Hv')".
+    iApply Match_InjR_wp.
+    iApply Let_wp. iApply Load_wp; iIntros "{$Hp} Hp". iApply Fst_wp.
+    iApply Let_wp. iApply Load_wp; iIntros "{$Hp} Hp". iApply Snd_wp.
+    iApply Op_wp. destruct (n =? 0) eqn: Hn.
+    + iApply If_true_wp. iApply Throw_Val_wp. iSplit; [done |].
+      iExists [], (n :: l'); simpl; eauto 6 with iFrame.
+    + iApply If_false_wp. iApply Seq_wp.
+      iApply Op_wp. iApply Pair_wp. iApply Store_wp; iIntros "{$Hp} Hp".
+      iApply ("IH" with "Hv'"); iSplit.
+      * iIntros (v) "[% Hv']".
+        replace (pred n) with (n - 1) by lia.
+        eauto with iFrame.
+      * iIntros (t v) "(% & %l1 & %l2 & -> & Hv')". iSplit; [done |].
+        iExists (n :: l1), l2; simpl.
+        replace (pred n) with (n - 1) by lia.
+        eauto 6 with iFrame.
+Qed.
